clean up is finished

code/experimental/P256/t.c
@@ -193,6 +193,52 @@ void pointDoubleTest(uint64_t * pointA)
    
 }
 
+
+
+void pointDoubleTest2(uint64_t * pointA)
+{
+   uint64_t* resultPoint = (uint64_t *) malloc (sizeof (uint64_t) * 12);
+   uint64_t* tempBuffer = (uint64_t *) malloc (sizeof (uint64_t) * 117);
+   pointToDomain(pointA, pointA);
+   point_add(pointA, pointA, resultPoint, tempBuffer);
+   norm(resultPoint, resultPoint, tempBuffer);
+
+   uint64_t * expectedResult = (uint64_t *) malloc (sizeof (uint64_t) * 12);
+   
+   expectedResult[0] = 12166265573283071317uL;
+   expectedResult[1] = 651836049588995208uL;
+   expectedResult[2] = 8576576477032308956uL;
+   expectedResult[3] = 14038888694816908229uL;
+
+   expectedResult[4] = 406750811229934272uL;
+   expectedResult[5] = 17370794130649372875uL;
+   expectedResult[6] = 6917402344331298187uL;
+   expectedResult[7] = 2808755901269482612uL;
+ 
+   expectedResult[8] = 1uL;
+   expectedResult[9] = 0uL;
+   expectedResult[10] = 0uL;
+   expectedResult[11] = 0uL;
+   
+   bool flag = true;
+   for (int i = 0; i< 12; i++)
+   {
+      flag = flag && ~(expectedResult[i] ^ resultPoint[i]);
+   }
+
+   if (flag)
+      printf("%s\n", "The test (point double2) is correct"); 
+   else
+      {
+         printf("%s\n", "The test has not passed");
+         printf("%s\n", "The expectedResult:");
+         print_uu_l(expectedResult, 12, false);
+         printf("%s\n", "The gotten result");
+         print_uu_l(resultPoint, 12, false);
+      }
+   
+}
+
 int main()
 {
    time_t t; 
@@ -238,6 +284,7 @@ int main()
    
    pointAddTest(basePoint, q);
    pointDoubleTest(basePoint);
+   pointDoubleTest2(basePoint);
   
    
 }
